ulib/FStar.Map.fst
@@ -97,6 +97,11 @@ let equal (#key:eqtype) (#value:Type) (m1:t key value) (m2:t key value) : Type0 
     F.feq m1.mappings m2.mappings /\
     S.equal m1.domain m2.domain
 
-let lemma_equal_intro #key #value m1 m2 = ()
+let lemma_equal_intro #key #value m1 m2 =
+  let aux (k:key) : Lemma (m1.mappings k == m2.mappings k /\ S.mem k m1.domain = S.mem k m2.domain) =
+    assert (sel m1 k == sel m2 k);
+    assert (contains m1 k = contains m2 k)
+  in
+  Classical.forall_intro aux
 let lemma_equal_elim #key #value m1 m2  = ()
 let lemma_equal_refl #key #value m1 m2  = ()
