ulib/FStar.FiniteSet.Base.fsti
@@ -136,7 +136,7 @@ val disjoint (#a: eqtype) (s1: set a) (s2: set a)
 ///
 /// var x: T :| x in s;
 
-val choose (#a: eqtype) (s: set a{exists x. {:nopattern} mem x s})
+val choose (#a: eqtype) (s: set a{exists x. {:pattern (mem x s)} mem x s})
   : GTot (x: a{mem x s})
 
 /// We add the utility functions `remove` and `notin`:
@@ -174,7 +174,7 @@ let empty_set_contains_no_elements_fact =
 let length_zero_fact =
   forall (a: eqtype) (s: set a).{:pattern cardinality s}
       (cardinality s = 0 <==> s == emptyset)
-    /\ (cardinality s <> 0 <==> (exists x. {:nopattern} mem x s))
+    /\ (cardinality s <> 0 <==> (exists x. {:pattern (mem x s)} mem x s))
     
 /// We represent the following Dafny axiom with `singleton_contains_argument_fact`:
 ///
