ulib/FStar.GhostSet.fsti
@@ -42,7 +42,7 @@ let disjoint (#a:Type) (s1: set a) (s2: set a) =
   equal (intersect s1 s2) empty
 
 (* ops *)
-type subset (#a:Type) (s1:set a) (s2:set a) :Type0 = forall x. {:nopattern} mem x s1 ==> mem x s2
+type subset (#a:Type) (s1:set a) (s2:set a) :Type0 = forall x. {:pattern (mem x s1)} mem x s1 ==> mem x s2
 
 (* Properties *)
 val mem_empty: #a:Type -> x:a -> Lemma
@@ -71,13 +71,13 @@ val mem_complement: #a:Type -> x:a -> s:set a -> Lemma
    [SMTPat (mem x (complement s))]
 
 val mem_subset: #a:Type -> s1:set a -> s2:set a -> Lemma
-   (requires (forall x. {:nopattern} mem x s1 ==> mem x s2))
+   (requires (forall x. {:pattern (mem x s1)} mem x s1 ==> mem x s2))
    (ensures (subset s1 s2))
    [SMTPat (subset s1 s2)]
 
 val subset_mem: #a:Type -> s1:set a -> s2:set a -> Lemma
    (requires (subset s1 s2))
-   (ensures (forall x. {:nopattern} mem x s1 ==> mem x s2))
+   (ensures (forall x. {:pattern (mem x s1)} mem x s1 ==> mem x s2))
    [SMTPat (subset s1 s2)]
 
 val comprehend_mem (#a: Type) (f: (a -> GTot bool)) (x: a) 
@@ -91,7 +91,7 @@ val mem_of_set (#a: eqtype) (f: Set.set a) (x: a)
 (* extensionality *)
 
 val lemma_equal_intro: #a:Type -> s1:set a -> s2:set a -> Lemma
-    (requires  (forall x. {:nopattern} mem x s1 = mem x s2))
+    (requires  (forall x. {:pattern (mem x s1)} mem x s1 = mem x s2))
     (ensures (equal s1 s2))
     [SMTPat (equal s1 s2)]
 
