ulib/FStar.Int.fsti
@@ -269,7 +269,7 @@ val ones_from_vec_lemma: #n:pos ->
 let nth (#n:pos) (a:int_t n) (i:nat{i < n}) : Tot bool = index (to_vec #n a) i
 
 val nth_lemma: #n:pos -> a:int_t n -> b:int_t n ->
-  Lemma (requires forall (i:nat{i < n}). {:nopattern} nth a i = nth b i)
+  Lemma (requires forall (i:nat{i < n}). {:pattern (nth a i)} nth a i = nth b i)
         (ensures a = b)
 
 (* Lemmas for constants *)
